cp, fix for lemmas

src/ocaml-output/FStar_Parser_Const.ml
@@ -330,6 +330,7 @@ let (binder_strictly_positive_attr : FStar_Ident.lident) =
   psconst "strictly_positive"
 let (no_auto_projectors_attr : FStar_Ident.lident) =
   psconst "no_auto_projectors"
+let (no_subtping_attr_lid : FStar_Ident.lident) = psconst "no_subtyping"
 let (well_founded_relation_lid : FStar_Ident.lident) =
   p2l ["FStar"; "WellFounded"; "well_founded_relation"]
 let (gen_reset : ((unit -> Prims.int) * (unit -> unit))) =
