src/ocaml-output/FStar_Tactics_Monad.ml
@@ -519,44 +519,46 @@ let (new_uvar :
       FStar_Syntax_Syntax.typ ->
         FStar_Syntax_Syntax.should_check_uvar FStar_Pervasives_Native.option
           ->
-          FStar_Compiler_Range.range ->
-            (FStar_Syntax_Syntax.term * FStar_Syntax_Syntax.ctx_uvar) tac)
+          FStar_Syntax_Syntax.ctx_uvar Prims.list ->
+            FStar_Compiler_Range.range ->
+              (FStar_Syntax_Syntax.term * FStar_Syntax_Syntax.ctx_uvar) tac)
   =
   fun reason ->
     fun env ->
       fun typ ->
         fun sc_opt ->
-          fun rng ->
-            let should_check =
-              match sc_opt with
-              | FStar_Pervasives_Native.Some sc -> sc
-              | uu___ ->
-                  ((let uu___2 =
-                      FStar_Compiler_Effect.op_Less_Bar
-                        (FStar_TypeChecker_Env.debug env)
-                        (FStar_Options.Other "2635") in
-                    if uu___2
-                    then
-                      let uu___3 = FStar_Syntax_Print.term_to_string typ in
-                      FStar_Compiler_Util.print1
-                        "Tactic introduced a strict uvar for %s\n" uu___3
-                    else ());
-                   FStar_Syntax_Syntax.Strict) in
-            let uu___ =
-              FStar_TypeChecker_Env.new_implicit_var_aux reason rng env typ
-                should_check FStar_Pervasives_Native.None in
-            match uu___ with
-            | (u, ctx_uvar, g_u) ->
-                let uu___1 =
-                  add_implicits g_u.FStar_TypeChecker_Common.implicits in
-                bind uu___1
-                  (fun uu___2 ->
-                     let uu___3 =
-                       let uu___4 =
-                         let uu___5 = FStar_Compiler_List.hd ctx_uvar in
-                         FStar_Pervasives_Native.fst uu___5 in
-                       (u, uu___4) in
-                     ret uu___3)
+          fun apply_uvar_deps ->
+            fun rng ->
+              let should_check =
+                match sc_opt with
+                | FStar_Pervasives_Native.Some sc -> sc
+                | uu___ ->
+                    ((let uu___2 =
+                        FStar_Compiler_Effect.op_Less_Bar
+                          (FStar_TypeChecker_Env.debug env)
+                          (FStar_Options.Other "2635") in
+                      if uu___2
+                      then
+                        let uu___3 = FStar_Syntax_Print.term_to_string typ in
+                        FStar_Compiler_Util.print1
+                          "Tactic introduced a strict uvar for %s\n" uu___3
+                      else ());
+                     FStar_Syntax_Syntax.Strict) in
+              let uu___ =
+                FStar_TypeChecker_Env.new_tac_implicit_var reason rng env typ
+                  should_check FStar_Pervasives_Native.None apply_uvar_deps in
+              match uu___ with
+              | (u, ctx_uvar, g_u) ->
+                  let uu___1 =
+                    add_implicits g_u.FStar_TypeChecker_Common.implicits in
+                  bind uu___1
+                    (fun uu___2 ->
+                       let uu___3 =
+                         let uu___4 =
+                           let uu___5 = FStar_Compiler_List.hd ctx_uvar in
+                           FStar_Pervasives_Native.fst uu___5 in
+                         (u, uu___4) in
+                       ret uu___3)
 let (mk_irrelevant_goal :
   Prims.string ->
     FStar_TypeChecker_Env.env ->
@@ -577,7 +579,7 @@ let (mk_irrelevant_goal :
               let uu___ =
                 new_uvar reason env typ
                   (FStar_Pervasives_Native.Some FStar_Syntax_Syntax.Strict)
-                  rng in
+                  [] rng in
               bind uu___
                 (fun uu___1 ->
                    match uu___1 with
