src/typechecker/FStar.TypeChecker.Env.fsti
@@ -462,6 +462,15 @@ val def_check_closed_in_env   : Range.range -> msg:string -> env -> term -> unit
 val def_check_guard_wf        : Range.range -> msg:string -> env -> guard_t -> unit
 val close_forall              : env -> binders -> term -> term
 
+val new_tac_implicit_var : string ->
+                           Range.range ->
+                           env ->
+                           typ ->
+                           should_check_uvar ->
+                           option ctx_uvar_meta_t ->
+                           list S.ctx_uvar ->
+                           (term * list (ctx_uvar * Range.range) * guard_t)
+
 val new_implicit_var_aux : string ->
                            Range.range ->
                            env ->
