ulib/FStar.Pervasives.fsti
@@ -1014,6 +1014,8 @@ val strictly_positive : unit
   *)
 val no_auto_projectors : unit
 
+val no_subtyping : unit
+
 (** Pure and ghost inner let bindings are now always inlined during
     the wp computation, if: the return type is not unit and the head
     symbol is not marked irreducible.
